mark-and-sweep/spec/GC.Spec.Sweep.fsti
@@ -27,12 +27,6 @@ let fp_in_heap (fp: U64.t) (g: heap) : prop =
   fp = 0UL \/ (U64.v fp >= U64.v mword /\ U64.v fp < heap_size /\
                U64.v fp % U64.v mword == 0 /\ Seq.mem (fp <: obj_addr) (objects zero_addr g))
 
-/// fp_in_heap implies fp can be coerced to obj_addr when non-null
-val fp_in_heap_elim : (fp: U64.t) -> (g: heap) ->
-  Lemma (requires fp_in_heap fp g /\ fp <> 0UL)
-        (ensures U64.v fp >= U64.v mword /\ U64.v fp < heap_size /\
-                 U64.v fp % U64.v mword == 0 /\ Seq.mem (fp <: obj_addr) (objects zero_addr g))
-
 /// ---------------------------------------------------------------------------
 /// Sweep Step: Process One Object
 /// ---------------------------------------------------------------------------
